crates/sui-prover/tests/inputs/quantifiers/filter_loop.ok.move
@@ -1,0 +1,31 @@
+// ensure that a code loop implementing `filter` can be proved.
+
+module 0x42::filter_loop_ok;
+
+use prover::prover::{ensures, invariant};
+use prover::vector_iter::{filter, filter_range};
+
+#[ext(pure)]
+fun is_odd(x: &u64): bool {
+    (*x) % 2 == 1
+}
+
+fun filter_odd(v: &vector<u64>): vector<u64> {
+    let mut i = 0;
+    let mut r = vector[];
+    invariant!(|| ensures(i <= v.length() && r == filter_range!(v, 0, i, |j| is_odd(j))));
+    while (i < v.length()) {
+        if (is_odd(&v[i])) {
+            r.push_back(v[i]);
+        };
+        i = i + 1;
+    };
+    r
+}
+
+#[spec(prove)]
+fun filter_odd_spec(v: &vector<u64>): vector<u64> {
+    let r = filter_odd(v);
+    ensures(r == filter!(v, |j| is_odd(j)));
+    r
+}
